theories/Math/BasicPosetTheory.v
@@ -1,0 +1,95 @@
+Require Import Coq.Classes.RelationClasses.
+Require Import Coq.Program.Basics.
+Require Import Coq.Relations.Relation_Definitions.
+Require Import Coq.Relations.Relation_Operators.
+Require Import Coq.Setoids.Setoid.
+Require Import DschingisKhan.Prelude.PreludeInit.
+Require Import DschingisKhan.Prelude.PreludeMath.
+
+Module BasicPosetTheory.
+
+  Import MathProps MathNotations MathClasses.
+
+  Global Notation " '\sup' X '=' sup_X " := (isSupremumOf sup_X X)
+    (in custom math_form_scope at level 6, sup_X custom math_term_scope at level 1, X custom math_term_scope at level 5).
+  Global Notation " x '`isUpperBoundOf`' X " := (isUpperBoundOf x X)
+    (in custom math_form_scope at level 6, x custom math_term_scope at level 1, X custom math_term_scope at level 5).
+  Global Notation " f '\monotonic' " := (preserves_leProp1 f)
+    (in custom math_form_scope at level 6, f custom math_term_scope at level 1, no associativity).
+  Global Notation " '\{' '\sup' Y ':' X '∈' Xs '\}' " := (ensemble_bind Xs (fun X => fun sup_Y => isSupremumOf sup_Y Y))
+    (in custom math_term_scope at level 0, Xs custom math_term_scope at level 5, X name, Y custom math_term_scope at level 1, no associativity).
+
+  Global Create HintDb poset_hints.
+  Global Hint Unfold REFERENCE_HOLDER isUpperBoundOf isSupremumOf isDirectedSubset : poset_hints.
+  Global Hint Resolve eqProp_Reflexive eqProp_Symmetric eqProp_Transitive : poset_hints.
+  Global Hint Resolve leProp_Reflexive leProp_Transitive eqProp_implies_leProp leProp_Antisymmetric : poset_hints.
+  Global Hint Resolve member_eq_leProp_with_impl member_eq_eqProp_with_iff : poset_hints.
+
+  Global Add Parametric Morphism (D : Type) (requiresPoset : isPoset D) :
+    (@isUpperBoundOf D requiresPoset) with signature (eqProp ==> eqProp ==> iff)
+    as UpperBound_compatWith_eqProp_WrtEnsembles.
+  Proof with eauto with *.
+    intros x y x_eq_y X Y X_eq_Y. split; intros H_upper_bound.
+    - intros z z_in_Y. rewrite <- x_eq_y. eapply H_upper_bound. unnw. rewrite -> X_eq_Y...
+    - intros z z_in_X. rewrite -> x_eq_y. eapply H_upper_bound. unnw. rewrite <- X_eq_Y...
+  Qed.
+
+  Global Hint Resolve UpperBound_compatWith_eqProp_WrtEnsembles : poset_hints.
+
+  Lemma supremum_monotonic_WrtEnsembles {D : Type} {requiresPoset : isPoset D}
+    (X1 : ensemble D) (X2 : ensemble D) (sup_X1 : D) (sup_X2 : D)
+    (sup_X1_isSupremumOf_X1 : $$ \sup X1 = sup_X1 $$)
+    (sup_X2_isSupremumOf_X2 : $$ \sup X2 = sup_X2 $$)
+    (X1_isSubsetOf_X2 : $$ X1 ⊆ X2 $$)
+    : $$ sup_X1 ≦ sup_X2 $$.
+  Proof.
+    eapply sup_X1_isSupremumOf_X1; ii.
+    eapply sup_X2_isSupremumOf_X2; eauto with *.
+  Qed.
+
+  Global Hint Resolve supremum_monotonic_WrtEnsembles : poset_hints.
+
+  Lemma supremum_preserves_eqProp_WrtEnsembles {D : Type} {requiresPoset : isPoset D}
+    (X1 : ensemble D) (X2 : ensemble D) (sup_X1 : D) (sup_X2 : D)
+    (sup_X1_isSupremumOf_X1 : $$ \sup X1 = sup_X1 $$)
+    (sup_X2_isSupremumOf_X2 : $$ \sup X2 = sup_X2 $$)
+    (X1_eq_X2 : $$ X1 ≡ X2 $$)
+    : $$ sup_X1 ≡ sup_X2 $$.
+  Proof.
+    pose proof (eqProp_implies_leProp X1 X2 X1_eq_X2) as claim1. symmetry in X1_eq_X2.
+    pose proof (eqProp_implies_leProp X2 X1 X1_eq_X2) as claim2. eapply leProp_Antisymmetric; eauto with *.
+  Qed.
+
+  Global Hint Resolve supremum_preserves_eqProp_WrtEnsembles : poset_hints.
+
+  Lemma Supremum_congruence {D : Type} {requiresPoset : isPoset D}
+    (sup_X : D) (sup_Y : D) (X : ensemble D) (Y : ensemble D)
+    (sup_X_eq_sup_Y : $$ sup_X ≡ sup_Y $$)
+    (X_eq_Y : $$ X ≡ Y $$)
+    (x_isSupremumOf_X : $$ \sup X = sup_X $$)
+    : $$ \sup Y = sup_Y $$.
+  Proof with eauto with *.
+    intros z. unnw. rewrite <- sup_X_eq_sup_Y. split.
+    - intros sup_X_le_z. rewrite <- X_eq_Y. eapply x_isSupremumOf_X...
+    - intros z_isUpperBoundOf_Y. eapply x_isSupremumOf_X. unnw. rewrite -> X_eq_Y...
+  Qed.
+
+  Global Hint Resolve Supremum_congruence : poset_hints.
+
+  Global Add Parametric Morphism (D : Type) (requiresPoset : isPoset D) :
+    (@isSupremumOf D requiresPoset) with signature (eqProp ==> eqProp ==> iff)
+    as Supremum_compatWith_eqProp_WrtEnsembles.
+  Proof. iis; eauto with *. Qed.
+
+  Lemma Supremum_in_SupremumMap {D : Type} {requiresPoset : isPoset D}
+    (X : ensemble D) (sup_X : D) (Xs : ensemble (ensemble D))
+    (sup_X_isSupremumOf_X : $$ \sup X = sup_X $$)
+    (X_in_Xs : $$ X ∈ Xs $$)
+    : $$ sup_X ∈ \{ \sup Xs_i : Xs_i ∈ Xs \} $$.
+  Proof.
+    exists (X). split.
+    - exact (X_in_Xs).
+    - exact (sup_X_isSupremumOf_X).
+  Qed.
+
+End BasicPosetTheory.
