theories/Prelude/LawOfExclusiveMiddle.v
@@ -1,0 +1,3 @@
+Require Import DschingisKhan.Prelude.PreludeInit.
+Require Import DschingisKhan.Prelude.PreludeMath.
+Require Import DschingisKhan.Prelude.PreludeUtil.
